\section*{1)} % (fold)

\subsection*{a)} % (fold)
\label{sub:a_}

We define the following operators: 

\begin{itemize}
	\item $\astrosun$ : element-wise multiplication
	\item $\otimes$ : dot product 
	\item $\oplus$ : element-wise sum
	\item $\sigma$ : sigmoid activation function
	\item $t$ : tanh activation function
\end{itemize}

Also we define the follwoing paramaters to be trained as:
\[
W, M \in \mathbb{R}^{m \times n}, b,d \in \mathbb{R}^{m}. 
\].

In addition $x \in \mathbb{R}^{n}$.

\begin{tikzpicture}[font=\small\sffamily,shorten >=1pt,->,auto,node distance=4cm,
semithick]


\tikzset{input_state/.style={state,    
                                 minimum size=1cm,
                                 minimum width=0.5cm,
                                 line width=0.5mm,
                                 fill=gray!80!white}}
  
\tikzset{param_state/.style={state,    
                                 minimum size=1cm,
                                 minimum width=0.5cm,
                                 line width=0.5mm,
                                 fill=gray!30!white}}

\tikzset{operator_state/.style={state,    
                                 minimum size=1cm,
                                 minimum width=0.5cm,
                                 line width=0.5mm}}

\node[param_state, ] (weight_W) {W};
\node[input_state, below = 3 of weight_W] (x) {x};
\node[param_state, below = 3 of x] (weight_M) {M};

\node[operator_state, below right = 1 and 1 of weight_W] (times_1) {$\otimes$};
\node[operator_state, below right = 1 and 1 of x] (times_2) {$\otimes$};

\node[operator_state, right = 2 of times_1] (sum_1) {$\oplus$};
\node[operator_state, right = 2 of times_2] (sum_2) {$\oplus$};

\node[param_state, right = 3 of weight_W] (b) {b};
\node[param_state, right = 3 of weight_M] (d) {d};

\node[param_state, right = 2 of sum_1] (tanh) {$t$};
\node[param_state, right = 2 of sum_2] (sigmoid) {$\sigma$};

\node[operator_state, below = 1 of tanh] (elem_wise) {$\astrosun$};

\node[param_state, right = 1 of elem_wise] (h) {h};

\begin{scope}[every node/.style={scale=0.75}]
	\path[->] (weight_W) edge node {} (times_1);                       
	\path[->] (x) edge node {} (times_1); 

	\path[->] (weight_M) edge node {} (times_2);                       
	\path[->] (x) edge node {} (times_2);

	\path[->] (times_1) edge node {} (sum_1);                       
	\path[->] (times_2) edge node {} (sum_2); 

	\path[->] (b) edge node {} (sum_1);                       
	\path[->] (d) edge node {} (sum_2); 

	\path[->] (sum_1) edge node {} (tanh);                       
	\path[->] (sum_2) edge node {} (sigmoid);

	\path[->] (tanh) edge node {} (elem_wise);                       
	\path[->] (sigmoid) edge node {} (elem_wise);

	\path[->] (elem_wise) edge node {} (h);
\end{scope}
\end{tikzpicture}
% subsection a_ (end)

\subsection*{b)} % (fold)
\label{sub:b_}

To make the calculation easier, we define some variables. 
To be sure $\textbf{A}_(i,j)$ presents the elemnent of the i-th row and 
the j-th column of matrix $\textbf{A}$.

We define: 

\newcommand{\zm}{\mathbf{z_m}}
\newcommand{\zw}{\mathbf{z_w}}
\newcommand{\yw}{\mathbf{y_w}}
\newcommand{\ym}{\mathbf{y_m}}
\newcommand{\pfr}[2]{\frac{\partial #1}{\partial #2}}

\begin{itemize}
	\item $\zw = \textbf{Wx} + \textbf{b}$
	\item $\zm = \textbf{Mx} + \textbf{d}$
	\item $\yw = tanh(\zw)$
	\item $\ym = \sigma (\zm)$
	\item $\mathbf{h} = \yw \astrosun \ym $
	\item $\mathbf{\delta} = \frac{\partial E}{\partial \mathbf{h}}$
\end{itemize}

Let's first derive $\pfr{E}{\mathbf{W}_{(i,j)}}$:

\[
\pfr{E}{\mathbf{W}_{(i,j)}} = \pfr{E}{\mathbf{h}_{(i)}}\pfr{\mathbf{h}_{(i)}}{\mathbf{W}_{(i,j)}} = \mathbf{\delta}_{(i)}\pfr{\yw_{(i)}}{\mathbf{W}_{(i,j)}}\ym{(i)} = \ym{(i)}\mathbf{\delta}_{(i)}\pfr{\yw_{(i)}}{\zw_{(i)}}\pfr{\zw_{(i)}}{\mathbf{W}_{(i,j)}}
\]

So deriving the different parts, we get: 

\begin{align*}
    \pfr{\yw_{(i)}}{\zw_{(i)}} &= (1 - tanh^2(\zw_{(i)})) \\
    \pfr{\zw_{(i)}}{\mathbf{W}_{(i,j)}} &= \mathbf{x}_{(j)}\\
\end{align*}

So finally: 

\[
\pfr{E}{\mathbf{W}_{(i,j)}} = \ym{(i)}\mathbf{\delta}_{(i)}(1 - tanh^2(\zw_{(i)}))\mathbf{x}_{(j)}
\]

Deriving $M_{(i,j)}$ follows the same logic. The only difference is that $\pfr{\ym_{(i)}}{\zw_{(i)}} = \sigma(\zm_{(i)}) (1 - \sigma(\zm_{(i)}))$ 
and we get $\pfr{E}{\mathbf{M}_{(i,j)}} = \yw{(i)}\mathbf{\delta}_{(i)}\sigma(\zm_{(i)}) (1 - \sigma(\zm_{(i)}))\mathbf{x}_{(j)}$.

Deriving $\pfr{E}{\mathbf{b}_{(i)}}$:

\[
\pfr{E}{\mathbf{b}_{(i)}} = \pfr{E}{\mathbf{h}_{(i)}}\pfr{\mathbf{h}_{(i)}}{\mathbf{b}_{(i)}} = \mathbf{\delta}_{(i)}\pfr{\yw_{(i)}}{\mathbf{b}_{(i)}}\ym{(i)} = \ym{(i)}\mathbf{\delta}_{(i)}\pfr{\yw_{(i)}}{\zm_{(i)}}\pfr{\zm_{(i)}}{\mathbf{b}_{(i)}}
\]

So instead of $\pfr{\zm_{(i)}}{\mathbf{W}_{(i,j)}} = \mathbf{x}_j$, we now have $\pfr{\zm_{(i)}}{\mathbf{b}_{(i)}} = 1$ 
and our final result looks like:

\[
\pfr{E}{\mathbf{b}_{(i)}} = \ym{(i)}\mathbf{\delta}_{(i)}(1 - tanh^2(\zw_{(i)}))
\]

Analogous for $\pfr{E}{\mathbf{d}_{(i)}}$, we get:

\[
\pfr{E}{\mathbf{d}_{(i)}} = \yw{(i)}\mathbf{\delta}_{(i)}\sigma(\zm_{(i)}) (1 - \sigma(\zm_{(i)}))
\]

% subsection b_ (end)

\subsection*{c)} % (fold)
\label{sub:c_}

Assuming that we have multiple layers, we need to perform multiple ``layer transformations''. Thus, x could also be intepreted 
as the output of the previous layer. So let's derive $\pfr{E}{\mathbf{x}_{(i)}}$:

The difference now is that $\pfr{E}{\mathbf{x}_{(i)}}$ depends not only on $\mathbf{h}_{(i)}$ but also on 
all the other $\mathbf{h}_{(j)}, j \ne i$. So we need to write:

\begin{align*}
    \pfr{E}{\mathbf{x}_{(i)}} &= \sum_j^m \pfr{E}{\mathbf{h}_{(j)}}\pfr{\mathbf{h}_{(j)}}{x_{(i)}} \\
    &= \sum_j^m \mathbf{\delta}_{(j)} (\pfr{\yw_{(j)}}{x_{(i)}}\ym_{(j)} + \pfr{\ym_{(j)}}{x_{(i)}}\yw_{(j)})\\
    &= \sum_j^m \mathbf{\delta}_{(j)} (\pfr{\yw_{(j)}}{\zw_{(j)}}\pfr{\zw_{(j)}}{x_{(i)}}\ym_{(j)} + \pfr{\ym_{(j)}}{\zm_{(j)}}\pfr{\zm_{(j)}}{x_{(i)}}\yw_{(j)}) \\
\end{align*}

Let's derive $\pfr{\zw_{(j)}}{x_{(i)}}$ and $\pfr{\zm_{(j)}}{x_{(i)}}$:
 
\begin{align*}
    \pfr{\zw_{(j)}}{x_{(i)}} &= \mathbf{W}_{(j,i)} \\
    \pfr{\zm_{(j)}}{x_{(i)}} &= \mathbf{M}_{(j,i)} \\
\end{align*}.

So we finally get: 

\[
\pfr{E}{\mathbf{x}_{(i)}} = \sum_j^m \mathbf{\delta}_{(j)} ((1 - tanh^2(\zw_{(j)}))\mathbf{W}_{(j,i)}\ym_{(j)} + \sigma(\zm_{(j)}) (1 - \sigma(\zm_{(j)}))\mathbf{M}_{(j,i)}\yw_{(j)})
\]

% subsection c_ (end)








