\section*{1)} % (fold)
\label{sec:1}
For given pdf $p(x)$, we need to calculate mean(1), variance(2), and verify the normalization constant(3). 
\begin{enumerate}
	\item $ \int_{-\infty}^{\infty}xp(x)dx$ \\
	\item $  \int_{-\infty}^{\infty}(x-\mu)^2p(x)dx$ \\
	\item $ \int_{-\infty}^{\infty}p(x)dx=1$\\
\end{enumerate}

\subsection*{Exercise 1a)} % (fold)
\label{subsection:Exercise 1a)}
\[
p(x)=
\begin{cases}
1/2a, \text{ if } x \in [-a, a], a \in	 R^+ \\
0 \text{ else } 
\end{cases}
\]
\begin{enumerate}
	\item \begin{align*} \int_{-\infty}^{\infty}xp(x)dx = \int_{-a}^{a}\frac{x}{2a}dx=0 
	\end{align*}	 \\
	\item 
	\begin{align*} 
		 \int_{-\infty}^{\infty}(x-\mu)^2p(x)dx &=  \int_{-a}^{a}\frac{x^2}{2a}dx \\ &= [\frac{x^3}{6a}]_{-a}^{a} = 2[\frac{x^3}{6a}]_{0}^{a} = \frac{a^2}{3}
	\end{align*} 
	\item 
	\begin{align*}   \int_{-\infty}^{\infty}p(x)dx &=  \int_{-a}^{a}\frac{1}{2a}dx \\ &= [\frac{x}{2a}]_{-a}^{a} = 2[\frac{x}{2a}]_{0}^{a} = 1
	\end{align*}
\end{enumerate}

\newpage
% subsection Exercise 1a) (end)
\subsection*{Exercise 1b)} % (fold)
\label{subsection:Exercise 1b)}
\[
p(x)= \frac{1}{\sqrt{2\pi\sigma^2}}e^\frac{-(x-\mu)^2}{2\sigma^2}
\]
	
	\subsubsection*{Mean} % (fold)
	\label{ssub:mean}
	
	% subsubsection mean (end)

	 \begin{align*} \int_{-\infty}^{\infty}xp(x)dx &= \int_{-\infty}^{\infty}\frac{x}{\sqrt{2\pi\sigma^2}}e^\frac{-(x-\mu)^2}{2\sigma^2}dx,  \\ 
	  (x \to x + \mu) 
	  &= \int_{-\infty}^{\infty}\frac{x+\mu}{\sqrt{2\pi\sigma^2}}e^\frac{-x^2}{2\sigma^2}dx \\ 
	  &= \int_{-\infty}^{\infty}\frac{x}{\sqrt{2\pi\sigma^2}}e^\frac{-x^2}{2\sigma^2}dx + \int_{-\infty}^{\infty}\frac{\mu}{\sqrt{2\pi\sigma^2}}e^\frac{-x^2}{2\sigma^2}dx \\ 
	  \text { (int. of odd func. over sym. interval )} 
	  &= 0 + \int_{-\infty}^{\infty}\frac{\mu}{\sqrt{2\pi\sigma^2}}e^\frac{-x^2}{2\sigma^2}dx \\
	  (x \to x \sigma, \text{ int. by sub., add } \sigma) 
	  &= \mu\int_{-\infty}^{\infty}\frac{\sigma}{\sqrt{2\pi\sigma^2}}e^{\frac{-x^2}{2}}dx \\ 
	  &= \frac{\mu}{\sqrt{2\pi}}\int_{-\infty}^{\infty}e^{\frac{-x^2}{2}}dx \\ 
	  &= \frac{\mu}{\sqrt{2\pi}}\sqrt{2\pi} \\ 
	  &= \mu\cdot1 = \mu \\
	\end{align*}

	\subsubsection*{Variance} % (fold)
	\label{ssub:variance}

	\begin{align*}  \int_{-\infty}^{\infty}(x-\mu)^2p(x)dx &=  \int_{-\infty}^{\infty}\frac{(x-\mu)^2}{\sqrt{2\pi\sigma^2}}e^\frac{-(x-\mu)^2}{2\sigma^2}dx \\ (x \to x + \mu) &= 
	\int_{-\infty}^{\infty}\frac{x^2}{\sqrt{2\pi\sigma^2}}e^\frac{-x^2}{2\sigma^2}dx \\ 
	(x \to x \sigma, \text{ int. by sub., add } \sigma)
	&= \int_{-\infty}^{\infty}\sigma\frac{(x\sigma)^2}{\sqrt{2\pi\sigma^2}}e^\frac{-(x\sigma)^2}{2\sigma^2}dx \\
    &= \frac{\sigma^2}{\sqrt{2\pi}}\int_{-\infty}^{\infty}x^2(e^\frac{-x^2}{2})dx \text { (int. by parts } u(x) = x, v'(x) = xe^\frac{-x^2}{2}\\ &=
	\frac{\sigma^2}{\sqrt{2\pi}}([-xe^{\frac{-x^2}{2}}]_{-\infty}^{\infty}-\int_{-\infty}^{\infty}-e^{\frac{-x^2}{2}}dx) \\ &=
	\frac{\sigma^2}{\sqrt{2\pi}}\int_{-\infty}^{\infty}e^{\frac{-x^2}{2}}dx \\ &=
	\frac{\sigma^2}{\sqrt{2\pi}}\sqrt{2\pi} \\ &=
	\sigma^2
	\end{align*} 

	\subsubsection*{Normalization} % (fold)
	\label{ssub:normalization}

	\begin{align*}   
	\int_{-\infty}^{\infty}p(x)dx &=  \int_{-\infty}^{\infty}\frac{1}{\sqrt{2\pi\sigma^2}}e^\frac{-(x-\mu)^2}{2\sigma^2}dx \\
	(x \to x \sigma + \mu, \text{ int. by sub., add } \sigma) 
	&= \int_{-\infty}^{\infty}\frac{1}{\sqrt{2\pi}}e^\frac{-(x)^2}{2}dx \\ 
	&= \frac{1}{\sqrt{2\pi}}\int_{-\infty}^{\infty}e^\frac{-(x)^2}{2}dx \\
	&= \frac{1}{\sqrt{2\pi}}\sqrt{2\pi} \\ 
	&= 1
	\end{align*}

% subsection Exercise 1b) (end)

% \subsection*{Exercise 1c)} % (fold)
% \label{subsection:Exercise 1c)}
% \[
% p(x)=
% \begin{cases}
% c\sqrt{a^2-x^2}, \text{ if } \left | x \right | < a, a \in R^+ \\
% 0 \text{ else } 
% \end{cases}
% \]

% \begin{enumerate}
% 	\item 
% 	\begin{align*} \int_{-\infty}^{\infty}xp(x)dx &= \int_{-a}^{a}cx\sqrt{a^2-x^2}dx \\ &= [\frac{c(a^2-x^2)^{\frac{3}{2}}}{3}]_{-a}^{a}
% 	\\ &= 0 
% 	\end{align*}	 
% 	\item 
% 	\begin{align*}  \int_{-\infty}^{\infty}(x-\mu)^2p(x)dx &=  \int_{-a}^{a}x^{2}c\sqrt{a^2-x^2}dx \\ &= 
% 	[\frac{c\left(a^4\arcsin\left(\frac{x}{\left|a\right|}\right)-2x\left(a^2-x^2\right)^\frac{3}{2}+a^2x\sqrt{a^2-x^2}\right)}{8}
% 	]_{-a}^{a} \\ &= 
% 	\frac{{\pi}a^4c}{8}
% 	\end{align*} 
% 	\item 
% 	\begin{align*}   
% 		\int_{-\infty}^{\infty}p(x)dx &= \int_{-a}^{a}c\sqrt{a^2-x^2}dx \\ &= [\frac{c\left(a^2\arcsin\left(\frac{x}{a}\right)+x\sqrt{a^2-x^2}\right)}{2}]_{-a}^{a}
% 		\\ &=
% 		 \frac{a^2c\pi}{2} \\ &= 1 \\
% 	\end{align*}
%    	normalization constant c is $c = \frac{2}{a^2\pi}$
% \end{enumerate}
% % subsection Exercise 1c) (end)

\subsection*{1c)} % (fold)
\label{subsection:1c Presented)}
\[
p(x)=
\begin{cases}
c\sqrt{a^2-x^2}, \text{ if } \left | x \right | < a, a \in R^+ \\
0 \text{ else } 
\end{cases}
\]

\begin{enumerate}
	\item 
	We introduce substitution variable  $\theta$ where $x = a\sin\theta$ and $dx = a\cos\theta d\theta$ within new boundary $-\frac{\pi}{2}<\theta<\frac{\pi}{2}$.  \\
	\begin{align*}   
	\int_{-\infty}^{\infty}p(x)dx &= \int_{-a}^{a}c\sqrt{a^2-x^2}dx \\ &=
	\int_{-\frac{\pi}{2}}^{\frac{\pi}{2}}c\sqrt{a^2-a^2\sin^{2}\theta}a\cos\theta d\theta \\ &= 
	\int_{-\frac{\pi}{2}}^{\frac{\pi}{2}}ca^2\cos^{2}\theta d\theta \\ &= 
	ca^2\int_{-\frac{\pi}{2}}^{\frac{\pi}{2}}\frac{1-cos2\theta}{2} d\theta \\ &= 
	\frac{ca^2}{2}[\theta]_{-\frac{\pi}{2}}^{\frac{\pi}{2}} + 0 \text{ (integration of odd function over symmetric interval)} \\ &= 
	\frac{a^2c\pi}{2} \\ &= 1 
	\end{align*}	 
	normalization constant c is $c = \frac{2}{a^2\pi}$
	\item 
	\begin{align*}   
	\int_{-\infty}^{\infty}xp(x)dx &= \int_{-a}^{a}cx\sqrt{a^2-x^2}dx
	\\ &= \int_{-a}^{a}\frac{2}{a^2\pi}x\sqrt{a^2-x^2}dx
    \\ &= 0  	\text { (integration of odd function within symetric interval) }
	\end{align*} 
	\item 
	\begin{align*}  
	\int_{-\infty}^{\infty}(x-\mu)^2p(x)dx &=  \int_{-a}^{a}x^{2}c\sqrt{a^2-x^2}dx 
	\\ &= \int_{-a}^{a}x^{2}\frac{2}{a^2\pi}\sqrt{a^2-x^2}dx 
	\\ &= \int_{-\frac{\pi}{2}}^{\frac{\pi}{2}}\frac{2}{a^2\pi}a^2\sin^2\theta  \sqrt{a^2-a^2\sin^{2}\theta}a\cos\theta d\theta 
	\\ &= \int_{-\frac{\pi}{2}}^{\frac{\pi}{2}}\frac{2}{\pi}\sin^2\theta a^2\cos^2\theta d\theta 
	\\ &= \frac{2a^2}{\pi}\int_{-\frac{\pi}{2}}^{\frac{\pi}{2}}\frac{(1+\cos2\theta)}{2} \frac{(1-\cos2\theta)}{2}d\theta 
	\\ &= \frac{2a^2}{\pi}\int_{-\frac{\pi}{2}}^{\frac{\pi}{2}}\frac{(1-\cos^22\theta)}{4} d\theta 
	\\ &= \frac{2a^2}{\pi}\int_{-\frac{\pi}{2}}^{\frac{\pi}{2}}\frac{(1-\cos4\theta)}{4\cdot2} d\theta
	\\ &= \frac{a^2}{4\pi}[\theta]_{-\frac{\pi}{2}}^{\frac{\pi}{2}} + 0 \text{ (integration of odd function over symmetric interval)}
	\\ &= -\frac{a^{2}}{4}
	\end{align*}
\end{enumerate}

% subsection 1c Presented) (end)
% section 1 (end)